Thanks to Larry Paulson for pointing out that tail-recursive functions don't need termination proofs to be admitted into HOL's logic. As a result, these files have been simplified.
Termination proofs (which are still needed by our methodology) can now
be integrated naturally into induction proofs (as shown in the first
example of decompiler_demoTheory, which used to be 35 lines long, but
is now only 14 lines long. The main lemma behind this advance is
TAILREC_PRE_THM in tailrecTheory.

examples/mc-logic/decompilerLib.sig
@@ -3,10 +3,10 @@ sig
 
     include helperLib
 
-    val decompile : decompiler_tools -> string -> term quotation -> thm * thm list
+    val decompile : decompiler_tools -> string -> term quotation -> thm * thm
 
-    val decompile_arm  : string -> term quotation -> thm * thm list
-    val decompile_ppc  : string -> term quotation -> thm * thm list
-    val decompile_ia32 : string -> term quotation -> thm * thm list
+    val decompile_arm  : string -> term quotation -> thm * thm
+    val decompile_ppc  : string -> term quotation -> thm * thm
+    val decompile_ia32 : string -> term quotation -> thm * thm
 
 end
