examples/mc-logic/tailrecScript.sml
@@ -1,6 +1,6 @@
 
 open HolKernel boolLib bossLib Parse;
-open pred_setTheory arithmeticTheory;
+open pred_setTheory arithmeticTheory whileTheory;
 
 val _ = new_theory "tailrec";
 
@@ -11,92 +11,51 @@ val op \\ = op THEN;
 (* ---- definitions ----- *)
 
 val TAILREC_PRE_def = Define `
-  TAILREC_PRE f1 (f2:'a->'b) guard precondition (x:'a) = 
-    ?inv R. inv x /\ WF R /\ (!y. inv y ==> precondition y) /\
-            !y. inv y /\ guard y ==> inv (f1 y) /\ R (f1 y) y`;
+  TAILREC_PRE f1 guard precondition (x:'a) = 
+    (!k. (!m. m < k ==> guard (FUNPOW f1 m x)) ==> precondition (FUNPOW f1 k x)) /\    
+    ?n. ~guard (FUNPOW f1 n x)`;
 
-val TAILREC = Defn.Hol_defn "TAILREC" `
-  TAILREC x = if TAILREC_PRE f1 (f2:'a->'b) guard p x /\ guard x then TAILREC (f1 x) else f2 x`;
+val TAILREC_def = Define `
+  TAILREC f1 (f2:'a->'b) g x = f2 (WHILE g f1 x)`;
+
 
 (* ---- theorems ---- *)
 
+val TAILREC_PRE_THM = store_thm("TAILREC_PRE_THM",
+  ``!f1 g p x. TAILREC_PRE f1 g p (x:'a) = p x /\ (g x ==> TAILREC_PRE f1 g p (f1 x))``,
+   REPEAT STRIP_TAC \\ EQ_TAC \\ REWRITE_TAC [TAILREC_PRE_def] \\ STRIP_TAC THENL [
+     STRIP_TAC THEN1 METIS_TAC [FUNPOW,DECIDE ``~(n < 0)``]
+     \\ REVERSE (REPEAT STRIP_TAC)
+     THEN1 (Cases_on `n` \\ FULL_SIMP_TAC std_ss [FUNPOW] \\ METIS_TAC [])
+     \\ Q.PAT_ASSUM `!kk. (!m. cc) ==> bb` 
+          (MATCH_MP_TAC o REWRITE_RULE [FUNPOW] o Q.SPEC `SUC k`)
+     \\ REPEAT STRIP_TAC
+     \\ Cases_on `m` \\ FULL_SIMP_TAC bool_ss [FUNPOW,DECIDE ``SUC m < SUC n = m < n``],    
+     REVERSE (Cases_on `g x`) THENL [     
+       REVERSE (REPEAT STRIP_TAC) 
+       THEN1 (Q.EXISTS_TAC `0` \\ ASM_SIMP_TAC std_ss [FUNPOW])
+       \\ Cases_on `k` \\ ASM_SIMP_TAC std_ss [FUNPOW]
+       \\ METIS_TAC [DECIDE ``0 < SUC n``,FUNPOW],
+       RES_TAC \\ REVERSE (REPEAT STRIP_TAC) THEN1 METIS_TAC [FUNPOW]
+       \\ Cases_on `k` \\ ASM_SIMP_TAC std_ss [FUNPOW]
+       \\ Q.PAT_ASSUM `!k. (!m. cc) ==> bb` MATCH_MP_TAC
+       \\ METIS_TAC [FUNPOW,DECIDE ``SUC m < SUC n = m < n``]]]);
+
 val TAILREC_PRE_INDUCT = store_thm("TAILREC_PRE_INDUCT",
-  ``!P. (!x. TAILREC_PRE f1 (f2:'a->'b) g p x /\ p x /\ g x /\ P (f1 x) ==> P x) /\
-        (!x. TAILREC_PRE f1 f2 g p x /\ p x /\ ~g x ==> P x) ==>
-        (!x. TAILREC_PRE f1 f2 g p x ==> P (x:'a))``,
-  NTAC 3 STRIP_TAC \\ REWRITE_TAC [TAILREC_PRE_def] \\ STRIP_TAC
-  \\ NTAC 4 (Q.PAT_ASSUM `f (x:'a)` MP_TAC)
-  \\ REWRITE_TAC [AND_IMP_INTRO,GSYM CONJ_ASSOC]   
-  \\ ONCE_REWRITE_TAC [CONJ_COMM] \\ REWRITE_TAC [GSYM AND_IMP_INTRO]   
-  \\ NTAC 2 STRIP_TAC \\ Q.SPEC_TAC (`x`,`x`)
-  \\ recInduct (UNDISCH (SPEC_ALL relationTheory.WF_INDUCTION_THM))  
-  \\ REPEAT STRIP_TAC \\ Cases_on `g x` THENL [
-    `inv' (f1 x) /\ R (f1 x) x` by METIS_TAC [TAILREC_PRE_def]
-    \\ Q.PAT_ASSUM `!x. TAILREC_PRE f1 f2 g p x /\ p x /\ g x /\ P (f1 x) ==> P x` MATCH_MP_TAC
-    \\ RES_TAC \\ ASM_SIMP_TAC bool_ss [TAILREC_PRE_def]
-    \\ Q.EXISTS_TAC `inv'` \\ Q.EXISTS_TAC `R` \\ METIS_TAC [],
-    Q.PAT_ASSUM `!x. TAILREC_PRE f1 f2 g p x /\ p x /\ ~g x ==> P x` MATCH_MP_TAC
-    \\ ASM_SIMP_TAC bool_ss [TAILREC_PRE_def]
-    \\ Q.EXISTS_TAC `inv'` \\ Q.EXISTS_TAC `R` \\ METIS_TAC []]);
-
-val TAILREC_PRE_STEP = prove(
-  ``TAILREC_PRE f1 (f2:'a->'b) g p x /\ p x /\ g x ==> TAILREC_PRE f1 (f2:'a->'b) g p (f1 x)``,
-  SIMP_TAC bool_ss [TAILREC_PRE_def] \\ REPEAT STRIP_TAC
-  \\ Q.EXISTS_TAC `inv'` \\ Q.EXISTS_TAC `R` \\ METIS_TAC []);
-
-val TAILREC_LEMMA = METIS_PROVE (map (DISCH_ALL) (Defn.eqns_of TAILREC))
-  ``(?R. (!x. TAILREC_PRE f1 (f2:'a->'b) g p x /\ g x ==> R (f1 x) x) /\ WF R) ==>
-    (TAILREC f1 f2 g p x = if TAILREC_PRE f1 (f2:'a->'b) g p x /\ g x 
-                          then TAILREC f1 f2 g p (f1 x) else f2 x)``;
-
-val TAILREC_def = store_thm("TAILREC_def",
-  ``TAILREC f1 f2 g p x = if TAILREC_PRE f1 (f2:'a->'b) g p x /\ g x 
-                          then TAILREC f1 f2 g p (f1 x) else f2 x``,
-  MATCH_MP_TAC TAILREC_LEMMA
-  \\ Q.EXISTS_TAC `(\x y. TAILREC_PRE f1 f2 g p y /\ p y /\ g y /\ (x = f1 y))`
-  \\ STRIP_TAC THENL [  
-    SIMP_TAC std_ss [] \\ SIMP_TAC std_ss [TAILREC_PRE_def] 
-    \\ REPEAT STRIP_TAC \\ RES_TAC,
-    SIMP_TAC std_ss [relationTheory.WF_EQ_INDUCTION_THM] \\ REPEAT STRIP_TAC
-    \\ REVERSE (Cases_on `TAILREC_PRE f1 f2 g p x`) THEN1 METIS_TAC []
-    \\ Q.PAT_ASSUM `TAILREC_PRE f1 f2 g p x` MP_TAC 
-    \\ Q.SPEC_TAC (`x`,`x`) \\ MATCH_MP_TAC TAILREC_PRE_INDUCT \\ METIS_TAC []]);
+  ``!P. (!x. TAILREC_PRE f1 g p x /\ p x /\ g x /\ P (f1 x) ==> P x) /\
+        (!x. TAILREC_PRE f1 g p x /\ p x /\ ~g x ==> P x) ==>
+        (!x. TAILREC_PRE f1 g p x ==> P (x:'a))``,
+  NTAC 4 STRIP_TAC \\ `?n. ~g (FUNPOW f1 n x)` by METIS_TAC [TAILREC_PRE_def]
+  \\ Q.PAT_ASSUM `~g (FUNPOW f1 n x)` MP_TAC
+  \\ Q.PAT_ASSUM `TAILREC_PRE f1 g p x` MP_TAC 
+  \\ Q.SPEC_TAC (`x`,`x`) \\ Induct_on `n`
+  THEN1 (REWRITE_TAC [FUNPOW] \\ REPEAT STRIP_TAC \\ METIS_TAC [TAILREC_PRE_THM])
+  \\ FULL_SIMP_TAC std_ss [FUNPOW] \\ REPEAT STRIP_TAC \\ METIS_TAC [TAILREC_PRE_THM]);
 
 val TAILREC_THM = store_thm("TAILREC_THM",
-  ``TAILREC_PRE f1 (f2:'a->'b) g p x ==>
-      (TAILREC f1 f2 g p x = if g x then TAILREC f1 f2 g p (f1 x) else f2 x)``,
-  METIS_TAC [TAILREC_def]);
-
-val TAILREC_PROOF = store_thm("TAILREC_PROOF",
-  ``(?m. (!y. P y /\ ~g y ==> p y /\ Q (f2 y)) /\
-         (!y. P y /\ g y ==> p y /\ P (f1 y) /\ m (f1 y) < (m y):num)) ==>
-    !x. P x ==> Q (TAILREC f1 f2 g p x) /\ TAILREC_PRE f1 (f2:'a->'b) g p x``,
-  REPEAT STRIP_TAC 
-  \\ `TAILREC_PRE f1 f2 g p x` by 
-    (REWRITE_TAC [TAILREC_PRE_def] \\ Q.EXISTS_TAC `P` \\ Q.EXISTS_TAC `measure m` 
-     \\ SIMP_TAC bool_ss [prim_recTheory.WF_measure,prim_recTheory.measure_def,
-          relationTheory.inv_image_def] \\ METIS_TAC [])
-  \\ Q.PAT_ASSUM `P x` MP_TAC \\ CONV_TAC (UNBETA_CONV ``x:'a``)
-  \\ Q.PAT_ASSUM `TAILREC_PRE f1 f2 g p x` MP_TAC
-  \\ MATCH_MP_TAC TAILREC_PRE_INDUCT  
-  \\ SIMP_TAC std_ss [] \\ METIS_TAC [TAILREC_def]);
-   
-val TAILREC_NONREC = store_thm("TAILREC_NONREC",
-  ``(TAILREC f1 f2 (\x.F) p x = f2 x) /\ (TAILREC_PRE f1 f2 (\x.F) p x = p x)``,
-  ONCE_REWRITE_TAC [TAILREC_def,TAILREC_PRE_def] \\ SIMP_TAC std_ss []
-  \\ REPEAT STRIP_TAC \\ EQ_TAC \\ REPEAT STRIP_TAC \\ RES_TAC
-  \\ Q.EXISTS_TAC `p` \\ Q.EXISTS_TAC `measure (\x. 0)`
-  \\ ASM_SIMP_TAC std_ss [prim_recTheory.WF_measure]);
-
-val TAILREC_PRE_IMP = store_thm("TAILREC_PRE_IMP", 
-  ``(!x. i x ==> p x) /\
-    (?f. !x. i x /\ g x ==> i ((f1:'a->'a) x) /\ f (f1 x) < ((f x):num)) ==>
-    (i x ==> TAILREC_PRE (f1:'a->'a) (f2:'a->'b) g p x)``,
-  REPEAT STRIP_TAC \\ REWRITE_TAC [TAILREC_PRE_def]
-  \\ Q.EXISTS_TAC `i` \\ Q.EXISTS_TAC `measure f`
-  \\ ASM_REWRITE_TAC [prim_recTheory.WF_measure]
-  \\ SIMP_TAC std_ss [prim_recTheory.measure_def,relationTheory.inv_image_def]   
-  \\ METIS_TAC []);
+  ``!f1 (f2:'a->'b) g x. TAILREC f1 f2 g x = if g x then TAILREC f1 f2 g (f1 x) else f2 x``,
+  REPEAT STRIP_TAC \\ CONV_TAC (RATOR_CONV (ONCE_REWRITE_CONV [TAILREC_def]))
+  \\ ONCE_REWRITE_TAC [WHILE] \\ REWRITE_TAC [TAILREC_def] \\ METIS_TAC []);
 
 
 val _ = export_theory();
